theories/TM/Basic/Mono.v
@@ -19,14 +19,14 @@ Section Mk_Mono.
     - apply fin.
   Defined.
 
-  Variable (F : finType) (Rmove : Rel (tape sig) (F * tape sig)).
+  Variable (F : finType) (R : Rel (tape sig) (F * tape sig)).
 
   Definition Mk_R_p : Rel (tapes sig 1) (F * tapes sig 1) :=
-      fun tps1 '(p, tps2) => Rmove (tps1[@Fin0]) (p, tps2[@Fin0]).
+      fun tps1 '(p, tps2) => R (tps1[@Fin0]) (p, tps2[@Fin0]).
 
 End Mk_Mono.
 
-Arguments Mk_R_p { sig F } ( Rmove ) x y /.
+Arguments Mk_R_p { sig F } ( R ) x y /.
 
 
 
