theories/TM/Code/BinNumbers/EncodeBinNumbers.v
@@ -3,7 +3,7 @@
 From Undecidability Require Import TM.Util.Prelim Code.
 From Undecidability Require Import ArithPrelim.
 From PslBase Require Export Bijection.
-Require Export BinNums. (* Warning: There also is a constructor called [N] for the type [move] *)
+Require Export BinNums. 
 
 
 (* We use Coq's standard types [positive] and [N] *)
