theories/TM/Hoare/HoareMult.v
@@ -1,0 +1,247 @@
+(** ** Multiplication *)
+
+From Undecidability Require Import ProgrammingTools.
+From Undecidability Require Import Hoare.Hoare.
+
+From Undecidability Require Import CaseNat.
+From Undecidability Require Import ArithRing. (* for [ring_simplify] *)
+
+Arguments mult : simpl never.
+Arguments plus : simpl never.
+
+
+(** *** Addition *)
+
+
+Definition Add_Step : pTM sigNat^+ (option unit) 2 :=
+  If (CaseNat @ [|Fin1|])
+     (Return (Constr_S @ [|Fin0|]) None)
+     (Return Nop (Some tt)).
+
+Definition Add_Step_steps : nat := 9.
+
+Definition Add_Step_size (a b : nat) : Vector.t (nat->nat) 2 :=
+  match b with
+  | 0 => [|id; id|]
+  | S b' => [|S; S|]
+  end.
+
+Lemma Add_Step_SpecT_space (a b : nat) (ss : Vector.t nat 2) :
+  TripleT
+    (tspec (withSpace (SpecVector [|Contains _ a; Contains _ b|]) ss))
+    Add_Step_steps
+    Add_Step
+    (fun yout =>
+       tspec
+         (withSpace match yout, b with
+                    | Some _, 0 => SpecVector [|Contains _ a; Contains _ b|]
+                    | None, S b' => SpecVector [|Contains _ (S a); Contains _ b'|]
+                    | _, _ => SpecFalse
+                    end
+         (appSize (Add_Step_size a b) ss))).
+Proof.
+  unfold Add_Step. eapply If_SpecT with (k3 := 0).
+  - hstep. (* This automatically calls [apply LiftTapes_SpecT_space; [smpl_dupfree | ]]. *)
+    cbn. apply CaseNat_SpecT_size.
+  - cbn. destruct b as [ | b']; cbn in *; auto. hsteps_cbn; cbn. auto.
+  - destruct b as [ | b']; cbn in *; auto.
+    hsteps. cbn. cbn. eauto.
+  - cbn. intros. destruct yout. (* reflexivity. unfold CaseNat_steps, Add_Step_steps. lia. *)
+    + reflexivity.
+    + unfold CaseNat_steps, Add_Step_steps. lia.
+Qed.
+
+Definition Add_Loop : pTM sigNat^+ unit 2 := While Add_Step.
+
+Definition Add_Loop_steps b := 9 + 10 * b.
+
+Fixpoint Add_Loop_size (a b : nat) : Vector.t (nat->nat) 2 :=
+  match b with
+  | O => Add_Step_size a b
+  | S b' => Add_Step_size a b >>> Add_Loop_size (S a) b'
+  end.
+
+Lemma Add_Loop_SpecT_size (a b : nat) (ss : Vector.t nat 2) :
+  TripleT
+    (tspec (withSpace (SpecVector [|Contains _ a; Contains _ b|]) ss))
+    (Add_Loop_steps b)
+    (Add_Loop)
+    (fun _ => tspec
+             (withSpace
+                (SpecVector [|Contains _ (a+b); Contains _ 0|])
+                (appSize (Add_Loop_size a b) ss))).
+Proof.
+  (** We have to add the space vector to the abstract state *)
+  eapply While_SpecT with (P := fun '(a,b,ss) => _) (Q := fun '(a,b,ss) => _) (R := fun '(a,b,ss) => _) (f := fun '(a,b,ss) => _) (g := fun '(a,b,ss) => _) (x := (a,b,ss));
+    clear a b ss; intros ((x,y),ss).
+    - apply Add_Step_SpecT_space.
+    - intros [] tmid tout H1 H2.
+      destruct y as [ | y']; cbn in *; auto.
+      replace (x+0) with x by lia. split; eauto.
+    - intros tin tmid H1 H2.
+      destruct y as [ | y']; cbn in *; auto.
+      eexists (S x, y', _); cbn. repeat split.
+      + eauto.
+      + unfold Add_Step_steps, Add_Loop_steps. lia.
+      + replace (S x + y') with (x + S y') by lia. auto.
+Qed.
+
+
+Definition Add : pTM sigNat^+ unit 4 :=
+  LiftTapes (CopyValue _) [|Fin1; Fin2|];; (* copy n to a *)
+  LiftTapes (CopyValue _) [|Fin0; Fin3|];; (* copy m to b *)
+  LiftTapes Add_Loop [|Fin2; Fin3|];; (* Main loop *)
+  LiftTapes (Reset _) [|Fin3|]. (* Reset b *)
+
+Definition Add_steps m n := 98 + 12 * n + 22 * m.
+
+Definition Add_space (a b : nat) : Vector.t (nat->nat) 4 :=
+  [|(*0*) id; (*1*) id; (*2*) CopyValue_size b >> Add_Loop_size b a @>Fin0;
+    (*3*) CopyValue_size a >> (Add_Loop_size b a @>Fin1) >> Reset_size 0 |].
+
+Lemma Add_SpecT_space (a b : nat) (ss : Vector.t nat 4) :
+  TripleT
+    (tspec (withSpace (SpecVector [|Contains _ a; Contains _ b; Void; Void|]) ss))
+    (Add_steps a b)
+    Add
+    (fun _ => tspec (withSpace (SpecVector [|Contains _ a; Contains _ b; Contains _ (a+b); Void|])
+                            (appSize (Add_space a b) ss))).
+Proof. (* The tactic [hstep] takes also takes care of moving [withSpace] to the head symbol of each precondition *)
+  unfold Add.
+  hstep. hstep.
+  apply CopyValue_SpecT_size.
+  cbn. intros _. cbn.
+  hstep. cbn. hstep. cbn. apply CopyValue_SpecT_size.
+  cbn. intros _. hstep. cbn. hstep. cbn. apply Add_Loop_SpecT_size.
+  cbn. intros _. hstep. cbn. apply Reset_SpecT_space.
+  cbn. intros _. replace (b+a) with (a+b) by lia. auto.
+  reflexivity. reflexivity.
+  unfold CopyValue_steps, Reset_steps, Add_Loop_steps, Add_steps. rewrite !Encode_nat_hasSize. lia.
+Qed.
+
+(** *** Multiplication *)
+
+
+Definition Mult_Step : pTM sigNat^+ (option unit) 5 :=
+  If (LiftTapes CaseNat [|Fin0|])
+     (Return (
+          LiftTapes Add [|Fin1; Fin2; Fin3; Fin4|];; (* Add(n, c, c') *)
+          LiftTapes (MoveValue _) [|Fin3; Fin2|]
+        ) (None)) (* continue *)
+     (Return Nop (Some tt)). (* break *)
+
+Definition Mult_Step_steps m' n c :=
+  match m' with
+  | O => 6
+  | _ => 168 + 33 * c + 39 * n
+  end.
+
+Definition Mult_Step_space m' n c : Vector.t (nat->nat) 5 :=
+  match m' with
+  | 0 => [|id; id; id; id; id|]
+  | S m'' => [| (*0*) S;
+               (*1*) Add_space n c @> Fin0; (* = [id] *)
+               (*2*) (Add_space n c @> Fin1) >> MoveValue_size_y (n+c) c;
+               (*3*) (Add_space n c @> Fin2) >> MoveValue_size_x (n+c);
+               (*4*) (Add_space n c @>Fin3)
+             |]
+  end.
+
+Lemma Mult_Step_SpecT_size m' n c ss :
+  TripleT
+    (tspec (withSpace (SpecVector [|Contains _ m'; Contains _ n; Contains _ c; Void; Void|]) ss))
+    (Mult_Step_steps m' n c)
+    (Mult_Step)
+    (fun yout =>
+       tspec
+         (withSpace
+            match yout, m' with
+            | Some _, 0 => SpecVector [|Contains _ m'; Contains _ n; Contains _ c; Void; Void|]
+            | None, S m'' => SpecVector [|Contains _ m''; Contains _ n; Contains _ (n+c); Void; Void|]
+            | _, _ => SpecFalse
+            end (appSize (Mult_Step_space m' n c) ss))).
+Proof.
+  eapply If_SpecT.
+  - hsteps.
+  - destruct m' as [ | m'']; cbn; auto.
+    hsteps. apply Add_SpecT_space. cbn. hsteps. cbn. apply MoveValue_SpecT_size. reflexivity. cbn. auto.
+  - destruct m' as [ | m'']; cbn; auto.
+    hsteps. auto.
+  - intros tin ymid tout HEnc H1. (* This part is the same *)
+    cbn. destruct ymid, m' as [ | m'']; cbn in *; auto.
+    unfold Mult_Step_steps, MoveValue_steps, CaseNat_steps, Add_steps. rewrite !Encode_nat_hasSize.
+    lia.
+Qed.
+
+
+Definition Mult_Loop := While Mult_Step.
+
+Fixpoint Mult_Loop_steps m' n c :=
+  match m' with
+  | O => S (Mult_Step_steps m' n c)
+  | S m'' => S (Mult_Step_steps m' n c) + Mult_Loop_steps m'' n (n + c)
+  end.
+
+
+Fixpoint Mult_Loop_size m' n c :=
+  match m' with
+  | 0 => Mult_Step_space m' n c (* [id;...;id] *)
+  | S m'' => Mult_Step_space m' n c >>> Mult_Loop_size m'' n (n+c)
+  end.
+
+Lemma Mult_Loop_SpecT_size m' n c ss :
+  TripleT
+    (tspec (withSpace (SpecVector [|Contains _ m'; Contains _ n; Contains _ c; Void; Void|]) ss))
+    (Mult_Loop_steps m' n c)
+    (Mult_Loop)
+    (fun _ => tspec (withSpace
+                    (SpecVector [|Contains _ 0; Contains _ n; Contains _ (m' * n + c); Void; Void|])
+                    (appSize (Mult_Loop_size m' n c) ss))).
+Proof.
+  eapply While_SpecT with (P := fun '(m',n,c,ss) => _) (Q := fun '(m',n,c,ss) => _) (R := fun '(m',n,c,ss) => _) (f := fun '(m,n,c,ss) => _) (g := fun '(m,n,c,ss) => _) (x := (m',n,c,ss));
+    clear m' n c ss; intros (((m',n),c),ss).
+  - apply Mult_Step_SpecT_size.
+  - cbn. intros _ tmid tout H1 H2. destruct m' as [ | m'']; cbn in *; auto.
+  - cbn. intros tin tmid H1 H2. destruct m' as [ | m'']; cbn in *; auto.
+    eexists (_,_,_,_). repeat split; eauto.
+    intros _ tout. replace (m'' * n + (n + c)) with (S m'' * n + c) by (ring_simplify; lia). auto.
+Qed.
+
+  
+Definition Mult : pTM sigNat^+ unit 6 :=
+  LiftTapes (CopyValue _) [|Fin0; Fin5|];; (* m' := m *)
+  LiftTapes (Constr_O) [|Fin2|];; (* c := 0 *)
+  LiftTapes Mult_Loop [|Fin5; Fin1; Fin2; Fin3; Fin4|];; (* Main loop *)
+  LiftTapes (Reset _) [|Fin5|]. (* Reset m'=0 *)
+
+
+Definition Mult_steps (m n : nat) : nat := 12 * m + Mult_Loop_steps m n 0 + 57.
+
+Definition Mult_size (m n : nat) : Vector.t (nat->nat) 6 :=
+  [|(*0*) id;
+    (*1*) Mult_Loop_size m n 0 @> Fin1;
+    (*2*) Constr_O_size >> Mult_Loop_size m n 0 @> Fin2;
+    (*3*) Mult_Loop_size m n 0 @> Fin3;
+    (*4*) Mult_Loop_size m n 0 @> Fin4;
+    (*5*) CopyValue_size m >> Mult_Loop_size m n 0 @> Fin0 >> Reset_size 0
+   |].
+
+Lemma Mult_SpecT_space (m n : nat) (ss : Vector.t nat 6) :
+  TripleT
+    (tspec (withSpace (SpecVector [|Contains _ m; Contains _ n; Void; Void; Void; Void|]) ss))
+    (Mult_steps m n)
+    (Mult)
+    (fun _ => tspec (withSpace (SpecVector [|Contains _ m; Contains _ n; Contains _ (m * n); Void; Void; Void|])
+                            (appSize (Mult_size m n) ss))).
+Proof.
+  unfold Mult.
+  hstep. hstep. cbn. 
+  apply CopyValue_SpecT_size.
+  cbn. intros _. hsteps.
+  cbn. intros _. hstep. cbn. hstep. cbn. apply Mult_Loop_SpecT_size.
+  cbn. intros. hstep. cbn. apply Reset_SpecT_space.
+  cbn. intros _ t. replace (m * n + 0) with (m * n) by lia. auto. (** Now it is fine! *)
+
+  reflexivity. reflexivity.
+  unfold Mult_steps. ring_simplify. unfold CopyValue_steps, Constr_O_steps, Reset_steps. rewrite !Encode_nat_hasSize. cbn. ring_simplify. reflexivity.
+Qed.
