theories/TM/Hoare/HoareStdLib.v
@@ -1,0 +1,732 @@
+(** ** Hoare Rules for Machines from [Code/] *)
+
+From Undecidability Require Import ProgrammingTools.
+From Undecidability Require Import Hoare.HoareLogic Hoare.HoareCombinators Hoare.HoareRegister Hoare.HoareTactics.
+
+
+(** *** Copy.v *)
+
+From Undecidability Require Import TM.Code.Copy.
+
+(** We give all rule variants here, because automation is forbidden for these machines *)
+
+
+(* TODO: [CopyValue_size] should be renamed, and this function should be moved to [Code.v] *)
+Definition CopyValue_sizefun {sigX X : Type} {cX : codable sigX X} (x : X) : Vector.t (nat->nat) 2 := [|id; CopyValue_size x|].
+
+Lemma CopyValue_SpecT_size (sig : finType) (sigX X : Type) (cX : codable sigX X) (I : Retract sigX sig) (x : X) (ss : Vector.t nat 2) :
+  TripleT (tspec (withSpace (SpecVector [|Contains _ x; Void|]) ss))
+          (CopyValue_steps x) (CopyValue _)
+          (fun _ => tspec (withSpace (SpecVector [|Contains _ x; Contains _ x|]) (appSize (CopyValue_sizefun x) ss))).
+Proof.
+  eapply Realise_TripleT.
+  - apply CopyValue_Realise.
+  - apply CopyValue_Terminates.
+  - intros tin [] tout H HEnc. cbn in *. 
+    specialize (HEnc Fin0) as HEnc0; specialize (HEnc Fin1) as HEnc1. cbn in *. 
+    cbn in *; simpl_vector in *; cbn in *.
+    modpon H. tspec_solve.
+  - intros tin k HEnc. cbn in *.
+    specialize (HEnc Fin0) as HEnc0; specialize (HEnc Fin1) as HEnc1.
+    cbn in *; simpl_vector in *; cbn in *. eauto.
+Qed.
+
+Lemma CopyValue_SpecT (sig : finType) (sigX X : Type) (cX : codable sigX X) (I : Retract sigX sig) (x : X) :
+  TripleT (tspec (SpecVector [|Contains _ x; Void|])) (CopyValue_steps x) (CopyValue _) (fun _ => tspec (SpecVector [|Contains _ x; Contains _ x|])).
+Proof. eapply TripleT_RemoveSpace. cbn. intros s. apply CopyValue_SpecT_size. Qed.
+
+Lemma CopyValue_Spec_size (sig : finType) (sigX X : Type) (cX : codable sigX X) (I : Retract sigX sig) (x : X) (ss : Vector.t nat 2) :
+  Triple (tspec (withSpace (SpecVector [|Contains _ x; Void|]) ss))
+         (CopyValue _)
+         (fun _ => tspec (withSpace (SpecVector [|Contains _ x; Contains _ x|]) (appSize (CopyValue_sizefun x) ss))).
+Proof. eapply TripleT_Triple. apply CopyValue_SpecT_size. Qed.
+
+Lemma CopyValue_Spec (sig : finType) (sigX X : Type) (cX : codable sigX X) (I : Retract sigX sig) (x : X) :
+  Triple (tspec (SpecVector [|Contains _ x; Void|]))
+         (CopyValue _)
+         (fun _ => tspec (SpecVector [|Contains _ x; Contains _ x|])).
+Proof. eapply Triple_RemoveSpace. apply CopyValue_Spec_size. Qed.
+
+
+
+Lemma Reset_SpecT_space (sig : finType) (sigX X : Type) (cX : codable sigX X) (I : Retract sigX sig) (x : X) (ss : Vector.t nat 1) :
+  TripleT (tspec (withSpace (SpecVector [|Contains _ x|]) ss)) (Reset_steps x) (Reset _) (fun _ => tspec (withSpace (SpecVector [|Void|]) (appSize [|Reset_size x|] ss))).
+Proof.
+  eapply Realise_TripleT.
+  - apply Reset_Realise.
+  - apply Reset_Terminates.
+  - intros tin [] tout H HEnc. cbn in *.
+    specialize (HEnc Fin0); cbn in *. simpl_vector in *; cbn in *.
+    modpon H.
+    
+
+    tspec_solve.
+  - intros tin k HEnc. cbn in *.
+    specialize (HEnc Fin0). simpl_vector in *; cbn in *. eauto.
+Qed.
+
+Lemma Reset_SpecT (sig : finType) (sigX X : Type) (cX : codable sigX X) (I : Retract sigX sig) (x : X) :
+  TripleT (tspec (SpecVector [|Contains _ x|])) (Reset_steps x) (Reset _) (fun _ => tspec (SpecVector [|Void|])).
+Proof. eapply TripleT_RemoveSpace. apply Reset_SpecT_space. Qed.
+
+Lemma Reset_Spec_size (sig : finType) (sigX X : Type) (cX : codable sigX X) (I : Retract sigX sig) (x : X) ss :
+  Triple (tspec (withSpace (SpecVector [|Contains _ x|]) ss)) (Reset _) (fun _ => tspec (withSpace (SpecVector [|Void|]) (appSize [|Reset_size x|] ss))).
+Proof. eapply TripleT_Triple. apply Reset_SpecT_space. Qed.
+
+Lemma Reset_Spec (sig : finType) (sigX X : Type) (cX : codable sigX X) (I : Retract sigX sig) (x : X) :
+  Triple (tspec (SpecVector [|Contains _ x|])) (Reset _) (fun _ => tspec (SpecVector [|Void|])).
+Proof. eapply TripleT_Triple. apply Reset_SpecT. Qed.
+
+
+Lemma ResetEmpty_SpecT_space (sig : finType) (sigX X : Type) (cX : codable sigX X) (I : Retract sigX sig) (x : X) (ss : Vector.t nat 1) :
+  cX x = [] ->
+  TripleT (tspec (withSpace (SpecVector [|Contains _ x|]) ss)) (ResetEmpty_steps) (ResetEmpty _) (fun _ => tspec (withSpace (SpecVector [|Void|]) (appSize [|ResetEmpty_size|] ss))).
+Proof.
+  intros HEncEmpty. eapply RealiseIn_TripleT.
+  - apply ResetEmpty_Sem.
+  - intros tin [] tout H HEnc. cbn in *.
+    specialize (HEnc Fin0); cbn in *. simpl_vector in *; cbn in *.
+    modpon H. tspec_solve.
+Qed.
+
+Lemma ResetEmpty_SpecT (sig : finType) (sigX X : Type) (cX : codable sigX X) (I : Retract sigX sig) (x : X) :
+  cX x = [] ->
+  TripleT (tspec (SpecVector [|Contains _ x|])) (ResetEmpty_steps) (ResetEmpty _) (fun _ => tspec (SpecVector [|Void|])).
+Proof. intros. eapply TripleT_RemoveSpace. intros. now apply ResetEmpty_SpecT_space. Qed.
+
+Lemma ResetEmpty_Spec_size (sig : finType) (sigX X : Type) (cX : codable sigX X) (I : Retract sigX sig) (x : X) ss :
+  cX x = [] ->
+  Triple (tspec (withSpace (SpecVector [|Contains _ x|]) ss)) (ResetEmpty _) (fun _ => tspec (withSpace (SpecVector [|Void|]) (appSize [|ResetEmpty_size|] ss))).
+Proof. intros. eapply TripleT_Triple. now apply ResetEmpty_SpecT_space. Qed.
+
+Lemma ResetEmpty_Spec (sig : finType) (sigX X : Type) (cX : codable sigX X) (I : Retract sigX sig) (x : X) :
+  cX x = [] ->
+  Triple (tspec (SpecVector [|Contains _ x|])) (ResetEmpty _) (fun _ => tspec (SpecVector [|Void|])).
+Proof. intros. eapply TripleT_Triple. now apply ResetEmpty_SpecT. Qed.
+
+
+Lemma ResetEmpty1_SpecT_space (sig : finType) (sigX X : Type) (cX : codable sigX X) (I : Retract sigX sig) (x : X) (ss : Vector.t nat 1) :
+  size cX x = 1 ->
+  TripleT (tspec (withSpace (SpecVector [|Contains _ x|]) ss)) (ResetEmpty1_steps) (ResetEmpty1 _) (fun _ => tspec (withSpace (SpecVector [|Void|]) (appSize [|ResetEmpty1_size|] ss))).
+Proof.
+  intros HEncEmpty. eapply RealiseIn_TripleT.
+  - apply ResetEmpty1_Sem.
+  - intros tin [] tout H HEnc. cbn in *.
+    specialize (HEnc Fin0); cbn in *. simpl_vector in *; cbn in *.
+    modpon H. tspec_solve.
+Qed.
+
+Lemma ResetEmpty1_SpecT (sig : finType) (sigX X : Type) (cX : codable sigX X) (I : Retract sigX sig) (x : X) :
+  size cX x = 1 ->
+  TripleT (tspec (SpecVector [|Contains _ x|])) (ResetEmpty1_steps) (ResetEmpty1 _) (fun _ => tspec (SpecVector [|Void|])).
+Proof. intros. eapply TripleT_RemoveSpace. intros. now apply ResetEmpty1_SpecT_space. Qed.
+
+Lemma ResetEmpty1_Spec_size (sig : finType) (sigX X : Type) (cX : codable sigX X) (I : Retract sigX sig) (x : X) ss :
+  size cX x = 1 ->
+  Triple (tspec (withSpace (SpecVector [|Contains _ x|]) ss)) (ResetEmpty1 _) (fun _ => tspec (withSpace (SpecVector [|Void|]) (appSize [|ResetEmpty1_size|] ss))).
+Proof. intros. eapply TripleT_Triple. now apply ResetEmpty1_SpecT_space. Qed.
+
+Lemma ResetEmpty1_Spec (sig : finType) (sigX X : Type) (cX : codable sigX X) (I : Retract sigX sig) (x : X) :
+  size cX x = 1 ->
+  Triple (tspec (SpecVector [|Contains _ x|])) (ResetEmpty1 _) (fun _ => tspec (SpecVector [|Void|])).
+Proof. intros. eapply TripleT_Triple. now apply ResetEmpty1_SpecT. Qed.
+
+
+
+(* TODO: Move to [Code/Copy.v] *)
+Definition MoveValue_size {X Y sigX sigY : Type} {cX : codable sigX X} {cY : codable sigY Y} (x : X) (y : Y) : Vector.t (nat->nat) 2 :=
+  [|MoveValue_size_x x; MoveValue_size_y x y|].
+
+Lemma MoveValue_SpecT_size (sig : finType) (sigX sigY X Y : Type)
+      (cX : codable sigX X) (cY : codable sigY Y) (I1 : Retract sigX sig) (I2 : Retract sigY sig) (x : X) (y : Y) (ss : Vector.t nat 2) :
+  TripleT (tspec (withSpace (SpecVector [|Contains _ x; Contains _ y|]) ss)) (MoveValue_steps x y) (MoveValue _)
+          (fun _ => tspec (withSpace (SpecVector [|Void; Contains _ x|]) (appSize (MoveValue_size x y) ss))).
+Proof.
+  eapply Realise_TripleT.
+  - apply MoveValue_Realise with (X := X) (Y := Y).
+  - apply MoveValue_Terminates with (X := X) (Y := Y).
+  - intros tin [] tout H HEnc. cbn in *.
+    specialize (HEnc Fin0) as HEnc0; specialize (HEnc Fin1) as HEnc1. simpl_vector in *; cbn in *.
+    modpon H. tspec_solve.
+  - intros tin k HEnc. cbn in *.
+    specialize (HEnc Fin0) as HEnc0; specialize (HEnc Fin1) as HEnc1. simpl_vector in *; cbn in *. eauto.
+Qed.
+
+Lemma MoveValue_SpecT (sig : finType) (sigX sigY X Y : Type)
+      (cX : codable sigX X) (cY : codable sigY Y) (I1 : Retract sigX sig) (I2 : Retract sigY sig) (x : X) (y : Y) :
+  TripleT (tspec (SpecVector [|Contains _ x; Contains _ y|])) (MoveValue_steps x y) (MoveValue _) (fun _ => tspec (SpecVector [|Void; Contains _ x|])).
+Proof. eapply TripleT_RemoveSpace. apply MoveValue_SpecT_size. Qed.
+
+Lemma MoveValue_Spec_size (sig : finType) (sigX sigY X Y : Type)
+      (cX : codable sigX X) (cY : codable sigY Y) (I1 : Retract sigX sig) (I2 : Retract sigY sig) (x : X) (y : Y) (ss : Vector.t nat 2) :
+  Triple (tspec (withSpace (SpecVector [|Contains _ x; Contains _ y|]) ss)) (MoveValue _)
+         (fun _ => tspec (withSpace (SpecVector [|Void; Contains _ x|]) (appSize (MoveValue_size x y) ss))).
+Proof. eapply TripleT_Triple. apply MoveValue_SpecT_size. Qed.
+
+Lemma MoveValue_Spec (sig : finType) (sigX sigY X Y : Type)
+      (cX : codable sigX X) (cY : codable sigY Y) (I1 : Retract sigX sig) (I2 : Retract sigY sig) (x : X) (y : Y) :
+  Triple (tspec (SpecVector [|Contains _ x; Contains _ y|])) (MoveValue _) (fun _ => tspec (SpecVector [|Void; Contains _ x|])).
+Proof. eapply TripleT_Triple. apply MoveValue_SpecT. Qed.
+
+
+Lemma Translate_SpecT_size (sig : finType) (sigX X : Type)
+      (cX : codable sigX X) (I1 I2 : Retract sigX sig) (x : X) (ss : Vector.t nat 1) :
+  TripleT (tspec (withSpace (SpecVector [|Contains I1 x|]) ss)) (Translate_steps x) (Translate I1 I2)
+          (fun _ => tspec (withSpace (SpecVector [|Contains I2 x|]) (appSize [|id|] ss))).
+Proof.
+  eapply Realise_TripleT.
+  - apply Translate_Realise with (X := X).
+  - apply Translate_Terminates with (X := X).
+  - intros tin [] tout H HEnc. cbn in *.
+    specialize (HEnc Fin0) as HEnc0; simpl_vector in *; cbn in *.
+    modpon H. tspec_solve.
+  - intros tin k HEnc Hk. cbn in *.
+    specialize (HEnc Fin0) as HEnc0. simpl_vector in *; cbn in *. unfold Translate_T. eauto.
+Qed.
+
+Lemma Translate_SpecT (sig : finType) (sigX X : Type)
+      (cX : codable sigX X) (I1 I2 : Retract sigX sig) (x : X) :
+  TripleT (tspec (SpecVector [|Contains I1 x|])) (Translate_steps x) (Translate I1 I2)
+          (fun _ => tspec (SpecVector [|Contains I2 x|])).
+Proof. eapply TripleT_RemoveSpace. apply Translate_SpecT_size. Qed.
+
+Lemma Translate_Spec_size (sig : finType) (sigX X : Type)
+      (cX : codable sigX X) (I1 I2 : Retract sigX sig) (x : X) (ss : Vector.t nat 1) :
+  Triple (tspec (withSpace (SpecVector [|Contains I1 x|]) ss)) (Translate I1 I2)
+         (fun _ => tspec (withSpace (SpecVector [|Contains I2 x|]) (appSize [|id|] ss))).
+Proof. eapply TripleT_Triple. apply Translate_SpecT_size. Qed.
+
+Lemma Translate_Spec (sig : finType) (sigX X : Type)
+      (cX : codable sigX X) (I1 I2 : Retract sigX sig) (x : X) :
+  Triple (tspec (SpecVector [|Contains I1 x|])) (Translate I1 I2)
+         (fun _ => tspec (SpecVector [|Contains I2 x|])).
+Proof. eapply TripleT_Triple. apply Translate_SpecT. Qed.
+
+
+(** We must not add these tactics to the automation! (As in [TM_Correct].) *)
+
+
+(** *** CompareValue *)
+
+(* TODO: s/CompareValues/CompareValue/g *)
+
+From Undecidability Require Import TM.Code.CompareValue.
+
+
+(* FIXME: I think we can also use [Triple_and_pre] and embed pure propositions into the postcondition. *)
+
+Section CompareValues.
+
+  Variable (sigX : finType) (X : eqType) (cX : codable sigX X).
+  Hypothesis (HInj : forall x y, cX x = cX y -> x = y).
+
+  Lemma CompareValue_SpecT_size (x y : X) (ss : Vector.t nat 2) :
+    TripleT (tspec (withSpace (SpecVector [|Contains _ x; Contains _ y|]) ss))
+            (CompareValues_steps x y) (CompareValues sigX)
+            (fun yout => tspec (withSpace (
+                                 match yout, Dec (x=y) with
+                                 | true,  Specif.left  _ => SpecVector [|Contains _ x; Contains _ y|]
+                                 | false, Specif.right _ => SpecVector [|Contains _ x; Contains _ y|]
+                                 | _, _ => SpecFalse
+                                 end) (appSize [|id; id|] ss))).
+  Proof.
+    eapply Realise_TripleT.
+    - now apply CompareValues_Realise.
+    - now apply CompareValues_TerminatesIn.
+    - intros tin yout tout H HEnc. cbn in *. 
+      specialize (HEnc Fin0) as HEnc0; specialize (HEnc Fin1) as HEnc1. cbn in *. 
+      cbn in *; simpl_vector in *; cbn in *.
+      modpon H. decide (x=y); subst; cbn in *.
+      + tspec_solve.
+      + tspec_solve.
+    - intros tin k HEnc Hk. cbn in *.
+      specialize (HEnc Fin0) as HEnc0; specialize (HEnc Fin1) as HEnc1.
+      cbn in *; simpl_vector in *; cbn in *.
+      unfold CompareValues_T. eauto.
+  Qed.
+
+  Lemma CompareValue_SpecT (x y : X) :
+    TripleT (tspec (SpecVector [|Contains _ x; Contains _ y|]))
+            (CompareValues_steps x y) (CompareValues sigX)
+            (fun yout => tspec (match yout, Dec (x=y) with
+                             | true,  Specif.left  _ => SpecVector [|Contains _ x; Contains _ y|]
+                             | false, Specif.right _ => SpecVector [|Contains _ x; Contains _ y|]
+                             | _, _ => SpecFalse
+                             end)).
+  Proof. eapply TripleT_RemoveSpace. cbn. intros s. apply CompareValue_SpecT_size. Qed.
+
+  Lemma CompareValue_Spec_size (x y : X) (ss : Vector.t nat 2) :
+    Triple (tspec (withSpace (SpecVector [|Contains _ x; Contains _ y|]) ss))
+           (CompareValues sigX)
+           (fun yout => tspec (withSpace (
+                                match yout, Dec (x=y) with
+                                | true,  Specif.left  _ => SpecVector [|Contains _ x; Contains _ y|]
+                                | false, Specif.right _ => SpecVector [|Contains _ x; Contains _ y|]
+                                | _, _ => SpecFalse
+                                end) (appSize [|id; id|] ss))).
+  Proof. eapply TripleT_Triple. apply CompareValue_SpecT_size. Qed.
+
+  Lemma CompareValue_Spec (x y : X) :
+    Triple (tspec (SpecVector [|Contains _ x; Contains _ y|]))
+           (CompareValues sigX)
+           (fun yout => tspec (match yout, Dec (x=y) with
+                            | true,  Specif.left  _ => SpecVector [|Contains _ x; Contains _ y|]
+                            | false, Specif.right _ => SpecVector [|Contains _ x; Contains _ y|]
+                            | _, _ => SpecFalse
+                            end)).
+  Proof. eapply Triple_RemoveSpace. apply CompareValue_Spec_size. Qed.
+
+End CompareValues.
+
+(** Again, no automation for this *)
+
+
+
+(** *** CaseNat *)
+
+From Undecidability Require Import TM.Code.CaseNat.
+
+(** Here, we only need to register the strongest version; the automation takes care of everything. *)
+
+Lemma Constr_O_SpecT_size (ss : Vector.t nat 1) :
+  TripleT (tspec (withSpace (SpecVector [|Void|]) ss)) Constr_O_steps Constr_O (fun _ => tspec (withSpace (SpecVector [|Contains _ 0|]) (appSize [|Constr_O_size|] ss))).
+Proof.
+  eapply RealiseIn_TripleT.
+  - apply Constr_O_Sem.
+  - intros tin [] tout H1 H2. cbn in *. specialize (H2 Fin0). simpl_vector in *; cbn in *. modpon H1. tspec_solve.
+Qed.
+
+Lemma Constr_S_SpecT_size :
+  forall (y : nat) ss,
+    TripleT (tspec (withSpace (SpecVector [|Contains _ y|]) ss)) Constr_S_steps Constr_S
+            (fun _ => tspec (withSpace (SpecVector [|Contains _ (S y)|]) (appSize [|S|] ss))).
+Proof.
+  intros y ss.
+  eapply RealiseIn_TripleT.
+  - apply Constr_S_Sem.
+  - intros tin [] tout H HEnc. cbn in *.
+    specialize (HEnc Fin0). simpl_vector in *; cbn in *. modpon H. tspec_solve.
+Qed.
+
+Definition CaseNat_size (n : nat) : Vector.t (nat->nat) 1 :=
+  match n with
+  | O => [|id|]
+  | S n' => [|S|]
+  end.
+
+Lemma CaseNat_SpecT_size (y : nat) (ss : Vector.t nat 1) :
+  TripleT
+    (tspec (withSpace (SpecVector [|Contains _ y|]) ss))
+    CaseNat_steps
+    CaseNat
+    (fun yout =>
+       tspec
+         (withSpace
+            (match yout, y with
+             | true, S y' => SpecVector [|Contains _ y'|]
+             | false, 0 => SpecVector [|Contains _ 0|]
+             | _, _ => SpecFalse
+             end)
+            (appSize (CaseNat_size y) ss))). (** Note that we add [withSpac] between the [tspec] and the [match] *)
+Proof.
+  eapply RealiseIn_TripleT.
+  - apply CaseNat_Sem.
+  - intros tin yout tout H HEnc. specialize (HEnc Fin0). simpl_vector in *; cbn in *. modpon H.
+    destruct yout, y; cbn in *; auto.
+    + tspec_solve.
+    + tspec_solve.
+Qed.
+
+Ltac hstep_Nat :=
+  lazymatch goal with
+  | [ |- TripleT ?P ?k Constr_O ?Q ] => eapply Constr_O_SpecT_size
+  | [ |- TripleT ?P ?k Constr_S ?Q ] => eapply Constr_S_SpecT_size
+  | [ |- TripleT ?P ?k CaseNat ?Q ] => eapply CaseNat_SpecT_size
+  end.
+
+Smpl Add hstep_Nat : hstep_smpl.
+
+
+(** *** CaseSum *)
+
+From Undecidability Require Import TM.Code.CaseSum.
+
+Section CaseSum.
+  Variable (X Y : Type) (sigX sigY : finType) (codX : codable sigX X) (codY : codable sigY Y).
+
+  Lemma Constr_inl_SpecT_size (x : X) (ss : Vector.t nat 1) :
+    TripleT
+      (tspec (withSpace (SpecVector [|Contains _ x|]) ss)) Constr_inl_steps (Constr_inl sigX sigY)
+      (fun _ => tspec (withSpace (SpecVector [|Contains _ (inl x)|]) (appSize [|pred|] ss))).
+  Proof.
+    eapply RealiseIn_TripleT.
+    - apply Constr_inl_Sem.
+    - intros tin [] tout H HEnc. cbn in *.
+      specialize (HEnc Fin0). simpl_vector in *; cbn in *. modpon H. tspec_solve.
+  Qed.
+
+  Lemma Constr_inr_SpecT_size (y : Y) (ss : Vector.t nat 1) :
+    TripleT
+      (tspec (withSpace (SpecVector [|Contains _ y|]) ss)) Constr_inr_steps (Constr_inr sigX sigY)
+      (fun _ => tspec (withSpace (SpecVector [|Contains _ (inr y)|]) (appSize [|pred|] ss))).
+  Proof.
+    eapply RealiseIn_TripleT.
+    - apply Constr_inr_Sem.
+    - intros tin [] tout H HEnc. cbn in *.
+      specialize (HEnc Fin0). simpl_vector in *; cbn in *. modpon H. tspec_solve.
+  Qed.
+
+  Lemma CaseSum_SpecT_size (s : X+Y) (ss : Vector.t nat 1) :
+    TripleT
+      (tspec (withSpace (SpecVector [|Contains _ s|]) ss)) (CaseSum_steps) (CaseSum sigX sigY)
+      (fun yout => tspec (withSpace
+                         (match yout, s with
+                          | true, inl x => SpecVector [|Contains _ x|]
+                          | false, inr y => SpecVector [|Contains _ y|]
+                          | _, _ => SpecFalse
+                          end)
+                         (appSize [|S|] ss))).
+  Proof.
+    eapply RealiseIn_TripleT.
+    - apply CaseSum_Sem.
+    - intros tin yout tout H HEnc. cbn in *.
+      specialize (HEnc Fin0). simpl_vector in *; cbn in *. modpon H.
+      destruct yout, s; cbn in *; auto; tspec_solve.
+  Qed.
+  
+End CaseSum.
+
+
+Section CaseOpton.
+  
+  Variable (X : Type) (sigX : finType) (codX : codable sigX X).
+
+  Lemma Constr_Some_SpecT_size (x : X) (ss : Vector.t nat 1) :
+    TripleT
+      (tspec (withSpace (SpecVector [|Contains _ x|]) ss)) Constr_Some_steps (Constr_Some sigX)
+      (fun _ => tspec (withSpace (SpecVector [|Contains _ (Some x)|]) (appSize [|pred|] ss))).
+  Proof.
+    eapply RealiseIn_TripleT.
+    - apply Constr_Some_Sem.
+    - intros tin [] tout H HEnc. cbn in *.
+      specialize (HEnc Fin0). simpl_vector in *; cbn in *. modpon H. tspec_solve.
+  Qed.
+
+  Lemma Constr_None_SpecT_size (ss : Vector.t nat 1) :
+    TripleT
+      (tspec (withSpace (SpecVector [|Void|]) ss)) Constr_None_steps (Constr_None sigX)
+      (fun _ => tspec (withSpace (SpecVector [|Contains _ None|]) (appSize [|pred|] ss))).
+  Proof.
+    eapply RealiseIn_TripleT.
+    - apply Constr_None_Sem.
+    - intros tin [] tout H HEnc. cbn in *.
+      specialize (HEnc Fin0). simpl_vector in *; cbn in *. modpon H. tspec_solve.
+  Qed.
+
+  Definition CaseOption_size (o : option X) : Vector.t (nat->nat) 1 :=
+    match o with
+    | None => [|CaseOption_size_None|]
+    | Some _ => [|CaseOption_size_Some|]
+    end.
+
+  Lemma CaseOption_SpecT_size (o : option X) (ss : Vector.t nat 1) :
+    TripleT
+      (tspec (withSpace (SpecVector [|Contains _ o|]) ss)) (CaseOption_steps) (CaseOption sigX)
+      (fun yout => tspec (withSpace
+                         (match yout, o with
+                          | true, Some x => SpecVector [|Contains _ x|]
+                          | false, None  => SpecVector [|Void|]
+                          | _, _ => SpecFalse
+                          end)
+                         (appSize (CaseOption_size o) ss))).
+  Proof.
+    eapply RealiseIn_TripleT.
+    - apply CaseOption_Sem.
+    - intros tin yout tout H HEnc. cbn in *.
+      specialize (HEnc Fin0). simpl_vector in *; cbn in *. modpon H.
+      destruct yout, o; cbn in *; auto; tspec_solve.
+  Qed.
+  
+End CaseOpton.
+
+
+Ltac hstep_Sum :=
+  match goal with
+  | [ |- TripleT ?P ?k (Constr_inl _ _) ?Q ] => eapply Constr_inl_SpecT_size
+  | [ |- TripleT ?P ?k (Constr_inr _ _) ?Q ] => eapply Constr_inr_SpecT_size
+  | [ |- TripleT ?P ?k (CaseSum    _ _) ?Q ] => eapply CaseSum_SpecT_size
+
+  | [ |- TripleT ?P ?k (Constr_Some _)  ?Q ] => eapply Constr_Some_SpecT_size
+  | [ |- TripleT ?P ?k (Constr_None _)  ?Q ] => eapply Constr_None_SpecT_size
+  | [ |- TripleT ?P ?k (CaseOption  _)  ?Q ] => eapply CaseSum_SpecT_size
+  end.
+
+Smpl Add hstep_Sum : hstep_smpl.
+
+
+(** *** CaseList *)
+
+From Undecidability Require Import TM.Code.CaseList.
+
+Section CaseList.
+
+  Variable (X : Type) (sigX : finType) (codX : codable sigX X).
+
+  Definition Constr_cons_sizefun (x : X) : Vector.t (nat->nat) 2 :=
+    [|Constr_cons_size x; id|].
+
+  Lemma Constr_cons_SpecT_size (x : X) (xs : list X) (ss : Vector.t nat 2) :
+    TripleT
+      (tspec (withSpace (SpecVector [|Contains _ xs; Contains _ x|]) ss)) (Constr_cons_steps x) (Constr_cons sigX)
+      (fun _ => tspec (withSpace (SpecVector [|Contains _ (x::xs); Contains _ x|]) (appSize (Constr_cons_sizefun x) ss))).
+  Proof.
+    eapply Realise_TripleT.
+    - apply Constr_cons_Realise.
+    - apply Constr_cons_Terminates.
+    - intros tin [] tout H HEnc. cbn in *.
+      specialize (HEnc Fin0) as HEnc0; specialize (HEnc Fin1) as HEnc1; simpl_vector in *; cbn in *.
+      modpon H. tspec_solve.
+    - intros tin k HEnc Hk. cbn.
+      specialize (HEnc Fin0) as HEnc0; specialize (HEnc Fin1) as HEnc1; simpl_vector in *; cbn in *.
+      eauto.
+  Qed.
+
+  Lemma Constr_nil_SpecT_size (ss : Vector.t nat 1) :
+    TripleT
+      (tspec (withSpace (SpecVector [|Void|]) ss)) Constr_nil_steps (Constr_nil sigX)
+      (fun _ => tspec (withSpace (SpecVector [|Contains _ nil|]) (appSize [|pred|] ss))).
+  Proof.
+    eapply RealiseIn_TripleT.
+    - apply Constr_nil_Sem.
+    - intros tin [] tout H HEnc. cbn in *.
+      specialize (HEnc Fin0). simpl_vector in *; cbn in *. modpon H. tspec_solve.
+  Qed.
+
+  Definition CaseList_size (xs : list X) : Vector.t (nat->nat) 2 :=
+    match xs with
+    | nil => [|id;id|]
+    | x :: xs => [|CaseList_size0 x; CaseList_size1 x|]
+    end.
+
+  Lemma CaseList_SpecT_size (xs : list X) (ss : Vector.t nat 2) :
+    TripleT
+      (tspec (withSpace (SpecVector [|Contains _ xs; Void|]) ss)) (CaseList_steps xs) (CaseList sigX)
+      (fun yout => tspec (withSpace
+                         (match yout, xs with
+                          | true,  x::xs' => SpecVector [|Contains _ xs'; Contains _ x|]
+                          | false,   nil => SpecVector [|Contains _ xs; Void|]
+                          | _, _ => SpecFalse
+                          end)
+                         (appSize (CaseList_size xs) ss))).
+  Proof.
+    eapply Realise_TripleT.
+    - apply CaseList_Realise.
+    - apply CaseList_Terminates.
+    - intros tin yout tout H HEnc. cbn in *.
+      specialize (HEnc Fin0) as HEnc0; specialize (HEnc Fin1) as HEnc1; simpl_vector in *; cbn in *.
+      modpon H. destruct yout, xs; cbn in *; eauto.
+      + destruct H as (H1&H2). tspec_solve.
+      + destruct H as (H1&H2). tspec_solve.
+    - intros tin k HEnc Hk. cbn.
+      specialize (HEnc Fin0) as HEnc0; specialize (HEnc Fin1) as HEnc1; simpl_vector in *; cbn in *.
+      eauto.
+  Qed.
+  
+
+End CaseList.
+
+
+Ltac hstep_List :=
+  match goal with
+  | [ |- TripleT ?P ?k (Constr_cons _) ?Q ] => eapply Constr_cons_SpecT_size
+  | [ |- TripleT ?P ?k (Constr_nil  _) ?Q ] => eapply Constr_nil_SpecT_size
+  | [ |- TripleT ?P ?k (CaseList    _) ?Q ] => eapply CaseList_SpecT_size
+  end.
+
+Smpl Add hstep_List : hstep_smpl.
+
+
+(** *** CasePair *)
+
+From Undecidability Require Import TM.Code.CasePair.
+
+Section CasePair.
+
+  Variable (X Y : Type) (sigX sigY : finType) (codX : codable sigX X) (codY : codable sigY Y).
+
+  Definition Constr_pair_sizefun (x : X) : Vector.t (nat->nat) 2 :=
+    [|id; Constr_pair_size x|].
+
+  Lemma Constr_pair_SpecT_size (x : X) (y : Y) (ss : Vector.t nat 2) :
+    TripleT (tspec (withSpace (SpecVector [|Contains _ x; Contains _ y|]) ss))
+            (Constr_pair_steps x) (Constr_pair sigX sigY)
+            (fun _ => tspec (withSpace (SpecVector [|Contains _ x; Contains _ (x,y)|])
+                                    (appSize (Constr_pair_sizefun x) ss))).
+  Proof.
+    eapply Realise_TripleT.
+    - apply Constr_pair_Realise.
+    - apply Constr_pair_Terminates.
+    - intros tin [] yout H HEnc.
+      specialize (HEnc Fin0) as HEnc0; specialize (HEnc Fin1) as HEnc1. simpl_vector in *; cbn in *. 
+      modpon H. simpl_vector in *. tspec_solve.
+    - intros tin k HEnc Hk.
+      specialize (HEnc Fin0) as HEnc0; specialize (HEnc Fin1) as HEnc1. simpl_vector in *; cbn in *. 
+      unfold Constr_pair_T. eauto.
+  Qed.
+
+  Definition CasePair_size (p : X*Y) : Vector.t (nat->nat) 2 :=
+    [| CasePair_size0 (fst p); CasePair_size1 (fst p) |].
+
+  Lemma CasePair_SpecT_size (p : X*Y) (ss : Vector.t nat 2) :
+    TripleT (tspec (withSpace (SpecVector [|Contains _ p; Void|]) ss))
+            (CasePair_steps (fst p)) (CasePair sigX sigY)
+            (fun _ => tspec (withSpace (SpecVector [|Contains _ (snd p); Contains _ (fst p)|])
+                                    (appSize (CasePair_size p) ss))).
+  Proof.
+    eapply Realise_TripleT.
+    - apply CasePair_Realise.
+    - apply CasePair_Terminates.
+    - intros tin [] tout H HEnc. cbn in *.
+      specialize (HEnc Fin0) as HEnc0; specialize (HEnc Fin1) as HEnc1. simpl_vector in *; cbn in *. 
+      modpon H. simpl_vector in *. tspec_solve.
+    - intros tin k HEnc Hk.
+      specialize (HEnc Fin0) as HEnc0; specialize (HEnc Fin1) as HEnc1. simpl_vector in *; cbn in *. 
+      unfold CasePair_T. eauto.
+  Qed.
+
+End CasePair.
+
+
+Ltac hstep_Pair :=
+  match goal with
+  | [ |- TripleT ?P ?k (Constr_pair _ _) ?Q ] => eapply Constr_pair_SpecT_size
+  | [ |- TripleT ?P ?k (CasePair    _ _) ?Q ] => eapply CasePair_SpecT_size
+  end.
+
+Smpl Add hstep_Pair : hstep_smpl.
+
+
+(** *** CaseFin *)
+
+From Undecidability Require Import TM.Code.CaseFin.
+
+
+(* FIXME: I am not sure about this one *)
+(* FIXME: [ChangeAlphabet] and [LiftTapes] don't support additional pure propositions, yet. *)
+(* TODO: We could write a custom rule for [hstep], like for [Return]. *)
+Section CaseFin.
+
+  Variable sig : finType.
+  Hypothesis defSig : inhabitedC sig.
+
+  (** A non-standard encoding! *)
+  Local Existing Instance Encode_Finite.
+
+  Definition CaseFin_size : Vector.t (nat->nat) 1 := [|S>>S|].
+
+  Lemma CaseFin_SpecT_size (x : sig) (ss : Vector.t nat 1) :
+    TripleT (tspec (withSpace (SpecVector [|Contains _ x|]) ss))
+            (CaseFin_steps) (CaseFin sig)
+            (fun yout tout => tspec (withSpace (SpecVector [|Void|]) (appSize CaseFin_size ss)) tout /\ yout = x).
+  Proof.
+    eapply RealiseIn_TripleT.
+    - apply CaseFin_Sem.
+    - intros tin yout tout H HEnc. cbn in *.
+      specialize (HEnc Fin0). simpl_vector in *; cbn in *. modpon H. split; auto. tspec_solve.
+  Qed.
+
+End CaseFin.
+
+(* TODO: For some reason, there is no constructor. It is just [WriteValue [x]]. *)
+
+Ltac hstep_Fin :=
+  match goal with
+  | [ |- TripleT ?P ?k (CaseFin _) ?Q ] => eapply CaseFin_SpecT_size
+  end.
+
+Smpl Add hstep_Pair : hstep_smpl.
+
+
+
+(** *** WriteValue *)
+
+(** [WriteValue] is a bit weird. See my thesis for the reason why. *)
+(* FIXME: The reason is obsolete (because there should be at most one encoding for each datatype and alphabet). *)
+From Undecidability Require Import TM.Code.WriteValue.
+
+Section WriteValue.
+
+  Variable (sig: finType) (X: Type) (cX: codable sig X).
+
+  Definition WriteValue_sizefun (x : X) : Vector.t (nat->nat) 1 := [| WriteValue_size x |].
+  
+  Lemma WriteValue_SpecT_size (x : X) (ss : Vector.t nat 1) :
+    TripleT (tspec (withSpace (SpecVector [|Void|]) ss))
+            (WriteValue_steps (size _ x)) (WriteValue (encode x))
+            (fun _ => tspec (withSpace (SpecVector [|Contains _ x|]) (appSize (WriteValue_sizefun x) ss))).
+  Proof.
+    eapply RealiseIn_TripleT.
+    - apply WriteValue_Sem.
+    - intros tin yout tout H HEnc. cbn in *.
+      specialize (HEnc Fin0). simpl_vector in *; cbn in *. modpon H. tspec_solve.
+  Qed.
+
+End WriteValue.
+
+Ltac hstep_WriteValue :=
+  match goal with
+  | [ |- TripleT ?P ?k (WriteValue _) ?Q ] => eapply WriteValue_SpecT_size
+  end.
+
+Smpl Add hstep_WriteValue : hstep_smpl.
+
+
+(** *** ListTM *)
+
+From Undecidability Require Import TM.Code.ListTM.
+
+(* TODO: Finally rename [Nth'] into [Nth] and delete all that commented obsolete code. *)
+Section Nth.
+
+  Variable (sig sigX : finType) (X : Type) (cX : codable sigX X).
+  Variable (retr1 : Retract (sigList sigX) sig) (retr2 : Retract sigNat sig).
+  Local Existing Instance retr_X_list'.
+
+  Lemma Nth'_SpecT_size (xs : list X) (n : nat) (ss : Vector.t nat 4) :
+    TripleT (tspec (withSpace (SpecVector [|Contains _ xs; Contains _ n; Void; Void|]) ss))
+            (Nth'_steps xs n) (Nth' retr1 retr2)
+            (fun yout =>
+               tspec (withSpace 
+                        (match yout, nth_error xs n with
+                         | true, Some x => SpecVector [|Contains _ xs; Void; Contains _ x; Void|]
+                         | false, None => SpecVector [|Contains _ xs; Void; Void; Void|]
+                         | _, _ => SpecFalse
+                         end) (appSize (Nth'_size xs n) ss))).
+  Proof.
+    eapply Realise_TripleT.
+    - apply Nth'_Realise.
+    - apply Nth'_Terminates.
+    - intros tin yout tout H HEnc. cbn in *.
+      specialize (HEnc Fin0) as HEnc0; specialize (HEnc Fin1) as HEnc1; specialize (HEnc Fin2) as HEnc2; specialize (HEnc Fin3) as HEnc3. simpl_vector in *; cbn in *. 
+      modpon H. destruct yout; cbn in *.
+      + destruct H as (x&H); modpon H. rewrite H. tspec_solve.
+      + modpon H. rewrite H. tspec_solve.
+    - intros tin k HEnc Hk.
+      specialize (HEnc Fin0) as HEnc0; specialize (HEnc Fin1) as HEnc1; specialize (HEnc Fin2) as HEnc2; specialize (HEnc Fin3) as HEnc3. simpl_vector in *; cbn in *. 
+      unfold Nth'_T. eauto 7.
+  Qed.
+
+End Nth.
+
+(* TODO: (Not needed for [Univ], but for [LM])
+- [Rev]
+- [App], [App']
+- [Length]
+*)
+
+Ltac hstep_ListTM :=
+  match goal with
+  | [ |- TripleT ?P ?k (Nth' _ _) ?Q ] => eapply Nth'_SpecT_size
+  end.
+
+Smpl Add hstep_ListTM : hstep_smpl.
