theories/TM/Univ/HoareUniv.v
@@ -1,0 +1,381 @@
+From Undecidability Require Import ProgrammingTools.
+From Undecidability Require Import Hoare.Hoare.
+From Undecidability Require Import Univ.LookupAssociativeListTM.
+From Undecidability Require Import Univ.HoareLookupAssociativeListTM.
+
+From Undecidability Require Import Univ.StepTM.
+From Coq Require Import ArithRing Lia.
+
+Section Univ.
+
+  (** Actually, we build a Universal Turing Machine for each alphabet [sigM] *)
+  Variable (sigM : finType).
+
+  Notation sigGraph := (sigList (sigPair (sigPair (option sigM) sigState) (sigPair (option sigM * move) sigState))).
+
+
+  (** We need to import all the Variables and Instances from the other file *)
+
+  (** The alphabet of [Univ] *)
+  Variable (sig : finType).
+  Variable (retr_sigGraph_sig : Retract sigGraph sig).
+  Variable (retr_sigTape_sig : Retract sigM sig).
+
+  (** Encoding of the current state number *)
+  Local Existing Instance StepTM.retr_sigCurrentStateNumber_sigGraph.
+  Local Existing Instance StepTM.retr_sigCurrentStateNumber_sig.
+
+  (** Encoding of the current state (= halt bit + number) *)
+  Local Existing Instance StepTM.retr_sigCurrentState_sigGraph.
+  Local Existing Instance StepTM.retr_sigCurrentState_sig.
+
+  (** Encoding of final bit of the current state *)
+  Local Existing Instance StepTM.retr_sigCurrentStateFinal_sigGraph.
+  Local Existing Instance StepTM.retr_sigCurrentStateFinal_sig.
+
+  (** Encoding of the next state *)
+  Local Existing Instance StepTM.retr_sigNextState_sigGraph.
+  Local Existing Instance StepTM.retr_sigNextState_sig.
+
+  (** Encoding the current symbol *)
+  Local Existing Instance StepTM.retr_sigCurrentSymbol_sigGraph.
+  Local Existing Instance StepTM.retr_sigCurrentSymbol_sig.
+
+  (** Encoding of actions *)
+  Local Existing Instance StepTM.retr_act_sigGraph.
+  Local Existing Instance StepTM.retr_act_sig.
+
+  (** Encoding of the keys for [Lookup] ([option sig * Q]) *)
+  Local Existing Instance StepTM.retr_key_sigGraph.
+  Local Existing Instance StepTM.retr_key_sig.
+
+  (** Encoding of the value for [Lookup] ([option sig * Q]) *)
+  Local Existing Instance StepTM.retr_value_sigGraph.
+  Local Existing Instance StepTM.retr_value_sig.
+
+
+  Local Existing Instance StepTM.Encode_graph.
+  Local Existing Instance StepTM.Encode_optSigM.
+  Local Existing Instance StepTM.Encode_action.
+
+
+  (** We have to define a [RegSpec] for [containsWorkingTape] *)
+
+  Definition ContainsWorkingTape (tp : tape sigM) : RegSpec sig :=
+    Custom (fun t => containsWorkingTape _ t tp).
+
+
+  (** The first high-level rule *)
+
+
+  Definition DoAction'_size (a : option sigM * move) : Vector.t (nat->nat) 2 :=
+    [| (*0*) id; (*1*) DoAction_size a |]. (** The entry for (*0*) is irrelevant, since it is a [Custom]. *)
+
+
+  (** The low-level machines are still verified using Realisation. The Hoare-framework doesn't make sense for low-level machines.
+      Thus, we just convert the relations to Hare triples. *)
+
+  Lemma DoAction'_SpecT_space (tp : tape sigM) (a : option sigM * move) ss :
+    TripleT (tspec (withSpace (SpecVector [|ContainsWorkingTape tp; Contains (StepTM.retr_act_sig _) a|]) ss))
+            (DoAction'_steps) (DoAction' _ _)
+            (fun _ => tspec (withSpace (SpecVector [|ContainsWorkingTape (doAct tp a); Void|]) (appSize (DoAction'_size a) ss))).
+  Proof.
+    unfold DoAction'_size; cbn. eapply RealiseIn_TripleT.
+    - apply DoAction'_Sem.
+    - cbn. intros tin _ tout H HEnc.
+      specialize (HEnc Fin0) as Henc0; specialize (HEnc Fin1) as HEnc1; cbn in *. unfold withSpace in *; simpl_vector in *; cbn in *.
+      modpon H. tspec_solve; eauto.
+  Qed.
+
+
+  Lemma SetFinal_SpecT_space (final : bool) (q : nat) ss :
+    TripleT (tspec (withSpace (SpecVector [|Contains (StepTM.retr_sigCurrentStateNumber_sig _) q; Void |]) ss))
+            (SetFinal_steps) (SetFinal _ final)
+            (fun yout => tspec
+                        (withSpace (SpecVector [|Contains (StepTM.retr_sigCurrentState_sig _) (final, q); Void|])
+                                   (appSize (SetFinal_size) ss))).
+  Proof.
+    eapply Realise_TripleT.
+    - apply SetFinal_Realise.
+    - apply SetFinal_Terminates.
+    - cbn. intros tin _ tout H HEnc.
+      specialize (HEnc Fin0) as Henc0; specialize (HEnc Fin1) as HEnc1; cbn in *. unfold withSpace in *; simpl_vector in *; cbn in *.
+      modpon H. tspec_solve; eauto.
+    - cbn. intros tin k HEnc Hk.
+      specialize (HEnc Fin0) as Henc0; specialize (HEnc Fin1) as HEnc1; cbn in *. unfold withSpace in *; simpl_vector in *; cbn in *.
+      hnf. eauto.
+  Qed.
+
+
+  Notation "'ContainsState' q" :=
+    (Contains (StepTM.retr_sigCurrentState_sig _) (halt q, index q)) (at level 0).
+
+  Notation "'ContainsState_size' q s" :=
+    (Contains_size (StepTM.retr_sigCurrentState_sig _) (halt q, index q) s) (at level 0).
+
+  Definition IsFinal_size' : Vector.t (nat->nat) 2 :=
+    [| (*0*) id; IsFinal_size |].
+
+  Lemma IsFinal_SpecT_space (M : TM sigM 1) (q : state M) ss :
+    TripleT (tspec (withSpace (SpecVector [|ContainsState q; Void|]) ss))
+            (IsFinal_steps (halt q)) (IsFinal _)
+            (fun yout =>
+               tspec
+                 (withSpace
+                    match yout, halt q with
+                    | true,  true  => SpecVector [|ContainsState q; Void|]
+                    | false, false => SpecVector [|ContainsState q; Void|]
+                    | _, _ => SpecFalse
+                    end (appSize (IsFinal_size') ss))).
+  Proof.
+    eapply Realise_TripleT.
+    - apply IsFinal_Realise.
+    - apply IsFinal_Terminates.
+    - intros tin yout tout H HEnc. cbn in *.
+      unfold containsState_size in *.
+      specialize (HEnc Fin0) as Henc0; specialize (HEnc Fin1) as HEnc1; cbn in *. unfold withSpace in *; simpl_vector in *; cbn in *.
+      modpon H. cbn in *. unfold containsState_size; eauto.
+      subst. destruct halt; cbn; auto; tspec_solve; eauto.
+    - cbn. intros tin k HEnc Hk.
+      specialize (HEnc Fin0) as Henc0; specialize (HEnc Fin1) as HEnc1; cbn in *. unfold withSpace in *; simpl_vector in *; cbn in *.
+      hnf. do 2 eexists. repeat split; eauto. unfold containsState. contains_ext.
+  Qed.
+
+
+  Definition ReadCurrent'_size : Vector.t (nat->nat) 2 :=
+    [| (*0*) id; ReadCurrent_size |].
+
+  Lemma ReadCurrent'_SpecT_space (tp : tape sigM) ss :
+    TripleT (tspec (withSpace (SpecVector [|ContainsWorkingTape tp; Void|]) ss))
+            (ReadCurrent'_steps) (ReadCurrent' _ _)
+            (fun _ => tspec (withSpace (SpecVector [|ContainsWorkingTape tp; Contains (StepTM.retr_sigCurrentSymbol_sig _) (current tp)|])
+                                    (appSize ReadCurrent'_size ss))).
+  Proof.
+    eapply RealiseIn_TripleT.
+    - apply ReadCurrent'_Sem.
+    - intros tin [] tout H HEnc.
+      specialize (HEnc Fin0) as Henc0; specialize (HEnc Fin1) as HEnc1; cbn in *. unfold withSpace in *; simpl_vector in *; cbn in *.
+      modpon H. tspec_solve; eauto.
+  Qed.
+
+
+
+  (** We now have rules for all auxiliary low-level machines of [Univ_Step], and can verify it now. *)
+
+  Notation "'ContainsTrans' M" :=
+    (Contains (retr_sigGraph_sig) (graph_of_TM M)) (at level 0).
+
+  Notation "'ContainsTrans_size' M s" :=
+    (Contains_size (retr_sigGraph_sig) (graph_of_TM M) s) (at level 0).
+
+  Local Arguments graph_of_TM : simpl never.
+
+  Lemma Univ_Step_SpecT_space (M : TM sigM 1) (tp : tape sigM) (q : state M) ss :
+    TripleT
+      (tspec (withSpace (SpecVector [|ContainsWorkingTape tp; ContainsTrans M; ContainsState q; Void; Void; Void|]) ss))
+      (Univ_Step_steps q tp) (Univ_Step _ _)
+      (fun yout =>
+         tspec (
+             withSpace
+               match yout, halt q with
+               | Some tt, true  => SpecVector [|ContainsWorkingTape tp;  ContainsTrans M; ContainsState q;  Void; Void; Void|]
+               | None,    false =>
+                 let (q', tp') := step (mk_mconfig q [|tp|]) in
+                 let tp' := tp'[@Fin0] in
+                 SpecVector [|ContainsWorkingTape tp'; ContainsTrans M; ContainsState q'; Void; Void; Void|]
+               | _, _ => SpecFalse
+               end
+               (appSize (Univ_Step_size tp q) ss))).
+  Proof.
+    unfold Univ_Step_size. cbn. destruct step eqn:HStep. cbn.
+    destruct (trans (q, [|current tp|])) as (q'&a) eqn:Etrans.
+    unfold step, current_chars in HStep. cbn in *. rewrite Etrans in HStep.
+    symmetry in HStep. inv HStep.
+
+    destruct (halt q) eqn:Ehalt; cbn in *.
+    - eapply If_SpecT with (k2 := Univ_Step_steps_IsFinal q tp) (k3 := Univ_Step_steps_IsFinal q tp). (* [halt q = true] *)
+      + hsteps_cbn. cbn.
+        eapply ConsequenceT_pre.
+        * apply IsFinal_SpecT_space with (q := q).
+        * cbn. intros. rewrite Ehalt. tspec_ext.
+        * reflexivity.
+      + cbn. rewrite Ehalt. cbn. hsteps_cbn.
+        apply Nop_SpecT_con; cbn; auto.
+        cbn. tspec_ext.
+      + cbn. rewrite Ehalt. cbn. eauto.
+      + cbn. intros ? ? ? _ _. destruct yout; auto.
+    - eapply If_SpecT with (k2 := Univ_Step_steps_IsFinal q tp) (k3 := Univ_Step_steps_IsFinal q tp). (* [halt q = false] *)
+      + hsteps_cbn. cbn.
+        eapply ConsequenceT_pre.
+        * apply IsFinal_SpecT_space with (q := q).
+        * cbn. rewrite <- Ehalt. tspec_ext.
+        * reflexivity.
+      + cbn. rewrite Ehalt. cbn. auto.
+      + rewrite Ehalt. cbn. hsteps_cbn; cbn.
+        apply ReadCurrent'_SpecT_space.
+        cbn. intros. tspec_ext.
+
+        cbn. eapply ConsequenceT_pre.
+        { apply Reset_SpecT_space with (I := StepTM.retr_sigCurrentSymbol_sig _). }
+        { instantiate (1 := [|_|]). cbn. tspec_ext. }
+        { reflexivity. }
+
+        eapply Lookup_SpecT_space.
+        { apply transition_graph_injective. }
+
+        cbn. tspec_ext.
+
+        cbn. intros .
+        rewrite <- Ehalt.
+        erewrite lookup_graph with (tp := tp).
+
+        (** We know that [Lookup] had succeeded. *)
+        rewrite Etrans; cbn.
+        destruct ymid; cbn in *; auto.
+
+        hstep; cbn. hstep; cbn. hstep; cbn. hstep; cbn.
+
+        instantiate (1 := (a[@Fin0], (halt q', index q'))). cbn. tspec_ext.
+
+        cbn. intros _. hstep; cbn. hstep; cbn. eapply ConsequenceT_pre.
+        { apply DoAction'_SpecT_space with (a := a[@Fin0]). }
+        { instantiate (1 := [|_;_|]). cbn. tspec_ext. }
+        { reflexivity. }
+
+        cbn. intros _. hstep; cbn. eapply ConsequenceT_pre.
+        { apply Translate_SpecT_size with (X := (bool * nat)%type). }
+
+        cbn. instantiate (1 := [|_|]). cbn. tspec_ext.
+        reflexivity. reflexivity. reflexivity. reflexivity. reflexivity. reflexivity.
+
+        (** The final runnint time calculation *)
+        {
+          unfold Univ_Step_steps_IsFinal. rewrite Ehalt, Etrans. cbn.
+          unfold Univ_Step_steps_ConstrPair, Univ_Step_steps_CasePair, Univ_Step_steps_Lookup, Univ_Step_steps_ResetSymbol, Univ_Step_steps_Translate.
+          rewrite <- !Ehalt. ring_simplify. set (Lookup_steps _ _). nia.
+        }
+
+        rewrite <- Ehalt.
+        cbn. tspec_ext. cbn. specialize (Htout Fin0). cbn in *. simpl_tape. auto.
+      + cbn. intros ? ? ? _ _. destruct yout; auto.
+  Qed.
+
+  
+  (** Version without space (actually needed later) *)
+  Lemma Univ_Step_SpecT (M : TM sigM 1) (tp : tape sigM) (q : state M) :
+    TripleT
+      (tspec (SpecVector [|ContainsWorkingTape tp; ContainsTrans M; ContainsState q; Void; Void; Void|]))
+      (Univ_Step_steps q tp) (Univ_Step _ _)
+      (fun yout =>
+         tspec 
+           match yout, halt q with
+           | Some tt, true  => SpecVector [|ContainsWorkingTape tp;  ContainsTrans M; ContainsState q;  Void; Void; Void|]
+           | None,    false =>
+             let (q', tp') := step (mk_mconfig q [|tp|]) in
+             let tp' := tp'[@Fin0] in
+             SpecVector [|ContainsWorkingTape tp'; ContainsTrans M; ContainsState q'; Void; Void; Void|]
+           | _, _ => SpecFalse
+           end).
+  Proof. eapply TripleT_RemoveSpace. apply Univ_Step_SpecT_space. Qed.
+
+
+
+  (** Partial correctness: If [Univ] terminates, so does [M] *)
+
+  Lemma tam (tp : tape sigM) a :
+    Vector.map2 (doAct (sig:=sigM)) [|tp|] a = [|doAct tp a[@Fin0]|].
+  Proof. destruct_vector. reflexivity. Qed.
+
+
+  Lemma Univ_Spec_space (M : TM sigM 1) (tp : tape sigM) (q : state M) ss :
+    Triple (tspec (withSpace (SpecVector [|ContainsWorkingTape tp; ContainsTrans M; ContainsState q; Void; Void; Void|]) ss))
+           (Univ _ _)
+           (fun _ tout =>
+              exists k (q' : state M) (tp' : tape sigM),
+                loopM (mk_mconfig q [|tp|]) k = Some (mk_mconfig q' [|tp'|]) /\
+                tspec (withSpace (SpecVector [|ContainsWorkingTape tp'; ContainsTrans M; ContainsState q'; Void; Void; Void|])
+                                 (appSize (Univ_size tp q k) ss))
+                      tout).
+  Proof.
+    eapply While_Spec with (P := fun '(tp,q,ss) => _) (Q := fun '(tp,q,ss) => _) (R := fun '(tp,q,ss) => _) (x := (tp,q,ss));
+      clear tp q ss; intros ((tp, q),ss); cbn in *.
+    - eapply TripleT_Triple. apply Univ_Step_SpecT_space.
+    - cbn. intros [] tmid tout H.
+      unfold step, current_chars; cbn.
+      destruct (halt q) eqn:Eh; auto. (* [halt q = true] *)
+      intros Hout. eexists 0, _, _; cbn. unfold haltConf. cbn. rewrite Eh. split.
+      + reflexivity.
+      + rewrite Eh. auto.
+    - cbn. intros tin tmid H1.
+      unfold step, current_chars; cbn. destruct trans as [q' a] eqn:Etrans. cbn.
+      destruct (halt q) eqn:Eh; auto. (* [halt q = false] *)
+
+      intros H2. rewrite tam in H2; cbn in *.
+      eexists (doAct tp a[@Fin0], q', _); cbn. split.
+      + tspec_ext.
+      + intros _ tout. intros (k&q''&tp''&Hloop&HEnc). eexists (S k), q'', tp''. repeat split.
+        * cbn. unfold haltConf. cbn. rewrite Eh. unfold step, current_chars. cbn. rewrite Etrans. rewrite tam. eauto.
+        * cbn. rewrite Eh. unfold step, current_chars. cbn. rewrite Etrans. cbn. rewrite !tam. cbn. tspec_ext.
+  Qed.
+
+
+  (** Complete Correctness: If [M] terminates, so does [Univ]. Note that we need a new triple for this. We also don't need spaces in this triple. *)
+
+  Lemma Univ_steps_eq (M : TM sigM 1) (q : state M) (tp : tape sigM) (k : nat) :
+    Univ_steps q tp k =
+    match k with
+    | 0 => Univ_Step_steps q tp
+    | S k' =>
+      if halt q
+      then Univ_Step_steps q tp
+      else let (q', tp') := step (mk_mconfig q [|tp|]) in
+           1 + Univ_Step_steps q tp + Univ_steps q' tp'[@Fin0] k'
+    end.
+  Proof. destruct k; cbn; auto. Qed.
+
+  Opaque Triple TripleT.
+
+  Lemma Univ_SpecT (M : TM sigM 1) (tp : tape sigM) (q : state M) (k' : nat) :
+    TripleT
+      (fun tin => exists (q' : state M) (tp' : tape sigM),
+           tspec (SpecVector [|ContainsWorkingTape tp; ContainsTrans M; ContainsState q; Void; Void; Void|]) tin /\
+           loopM (mk_mconfig q [|tp|]) k' = Some (mk_mconfig q' [|tp'|]))
+      (Univ_steps q tp k') (Univ _ _)
+      (fun _ tout =>
+         exists (q' : state M) (tp' : tape sigM),
+           loopM (mk_mconfig q [|tp|]) k' = Some (mk_mconfig q' [|tp'|]) /\
+           tspec (SpecVector [|ContainsWorkingTape tp'; ContainsTrans M; ContainsState q'; Void; Void; Void|]) tout).
+  Proof.
+    eapply While_SpecT with (P := fun '(tp,q,k') => _) (Q := fun '(tp,q,k') => _) (R := fun '(tp,q,k') => _)
+                            (f := fun '(tp,q,k') => _) (g := fun '(tp,q,k') => Univ_Step_steps q tp)
+                            (x := (tp,q,k'));
+      clear tp q k'; intros ((tp, q),k'); cbn in *.
+    - do 2 (eapply TripleT_exists_pre; intros). eapply TripleT_and_pre; intros _. (* First remove the pure preconditions *)
+      (* eapply TripleT_RemoveSpace. apply Univ_Step_SpecT_space. *)
+      apply Univ_Step_SpecT. (* Here we need the version without space again. *)
+    - cbn. intros [] tmid tout (q'&tp'&HEnc&HLoop).
+      unfold step, current_chars; cbn.
+      destruct (halt q) eqn:Eh; auto. (* [halt q = true] *)
+      intros Hout. repeat split.
+      + exists q', tp'. cbn. unfold haltConf; cbn.
+        apply loop_eq_0 in HLoop as HLoop'; eauto. inv HLoop'. rewrite Eh. split; auto.
+      + rewrite Univ_steps_eq. destruct k'; auto. rewrite Eh. reflexivity.
+    - intros tin tmid (q'&tp'&HEnc&HLoop). cbn.
+      unfold step, current_chars; cbn. destruct trans as [q'' a] eqn:Etrans. cbn.
+      destruct (halt q) eqn:Eh; auto. (* [halt q = false] *)
+
+      destruct k' as [ | k'']; cbn in *; unfold haltConf in HLoop; cbn in *; rewrite Eh in HLoop. congruence.
+      unfold step, current_chars in HLoop. cbn in *. rewrite Etrans in HLoop. rewrite tam in HLoop. cbn in *.
+
+      intros H2. exists (doAct tp a[@Fin0], q'', k''). repeat split.
+      + eexists q', tp'. repeat split; auto. tspec_ext. rewrite tam in H; cbn in *. eauto.
+      + rewrite Eh. cbn. unfold step, current_chars. cbn. rewrite Etrans. cbn. rewrite tam. cbn. reflexivity.
+      + cbn. intros _ tout (q'''&tp'''&HLoop'&HEnc').
+        apply (loop_injective HLoop) in HLoop'. inv HLoop'.
+        eexists _, _. repeat split.
+        * cbn. unfold haltConf; cbn. rewrite Eh. unfold step, current_chars; cbn. rewrite Etrans. rewrite tam. cbn. eauto.
+        * eauto.
+  Qed.
+
+
+End Univ.
